# Algebra 20220928

[TOC]

## Homomorphisms

$f: G\rightarrow G'$.    $\forall a,b\in G, f(ab)=f(a)f(b)$

$\ker (f) = \{g\in G|f(g)=1'\}$

$Im(f)=\{f(g)\in G'|g\in G\}$

==Note==: $\ker (f)=\{1\}\iff f \text{ is injective}$



## Conjugation

### Observation

$\ker(f)$ is a subgroup of $G$.

$\forall g \in G$,  $\forall x \in \ker(f)$, consider $gxg^{-1}\in G$

$f(gxg^{-1}) = f(g)f(x)f(g^{-1}) = f(g)\cdot 1'\cdot f(g^{-1}) = 1'$

So $gxg^{-1}\in \ker(f)$

### Definition

$G$ is a group, $x\in G, g\in G.$  The <u>**conjugation**</u> of $x$ by $g$ is the elemnt $gxg^{-1}$

### Conjugacy Class

We can define a relation on $G$ by $a\sim b$ if $\exist g\in G, b=gag^{-1}$. 

This can be verified to be an equivalence relation:

* $\forall a\in G,\ a = 1\cdot a \cdot 1',\ a\sim a$

* $$
    \begin{align*}
    &a\sim b\\
    \Rightarrow \quad &\exists g \in G, b=gag^{-1}\\
    \Rightarrow \quad   &a= g^{-1}bg=g^{-1}b(g^{-1})^{-1}\\
    \Rightarrow \quad   &b\sim a
    \end{align*}
    $$

* $$
    \begin{align*}
    &a\sim b, b\sim c\\
    \Rightarrow \quad  &\exists g_1 \in G, b=g_1ag_1^{-1}, \quad\exists g_2 \in G, c=g_2bg_2^{-1}\\
    \Rightarrow \quad  &c= g_2bg_2^{-1}=g_2(g_1ag_1^{-1})g_2^{-1} = (g_2g_1)a(g_2g_1)^{-1}\\
    \Rightarrow \quad   &a\sim c
    \end{align*}
    $$

Under this equivalence relation, if $a\sim b$, we say $a,b $ are conjugates, each equivalence class isi called a **<u>conjugracy class</u>**: $[a]=\{gag^{-1}\in G|g\in G\}$



## Normal Subgroup

### Definition

A subgroup $N$ of $G$ is called a normal subgroup if $\forall n \in N, \forall g \in G, $   $gng^{-1}\in N$.  (i.e., "closed under conjugation")

### Prop

The following statements are euqivalent for a subgroup $N$ of $G$:

1. $N$ is a normal subgroup of $G$
2. $\forall g\in G, gNg^{-1}=\{gng^{-1}\in G|g\in G, n\in N  \}\subseteq N$
3. $\forall g\in G, gNg^{-1}=N$

#### Proof

$(1)\iff(2)$ obvious by definition

$(3)\Rightarrow (2)$ obvious

$(2)\Rightarrow(3)$  
$$
\begin{align*}
\forall g \in G, gNg^{-1} &\subseteq N\\
g^{-1}(gNg^{-1})g &\subseteq g^{-1}Ng\\
N &\subseteq g^{-1}Ng = g^{-1}N(g^{-1})^{-1}\\
\text{i.e.}\qquad \forall g\in G, \ N&\subseteq gNg^{-1} \\
\text{so,  }\quad \qquad gNg^{-1} &= N
\end{align*}
$$

### Example

1. The motivation example:

    * for any homomorphism $f:G\rightarrow G'$

    * $\ker(f)$ is a normal subgroup of $G$.

    For example:

    * $\det: GL_n(\R) \rightarrow \R^x$

        > $\R^x$: the group of nonzero real numbers with multiplication

    * $\det$ is a homomorphism:

    * We know from Linear Algebra that $\det (AB) = \det(A)\cdot \det(B)$

    * $\ker(\det) = \{A\in GL_n(\R)|\det A = 1 \} = SL_n(\R)$

    * We can conclude $SL_n(\R)$ is a normal subgroup of $GL_n(\R)$

2. $G$ is abelian, then any subgroup $H$ of $G$ is a normal subgroup:

    * $\forall h \in H$,  $\forall g \in G$,  $ghg^{-1}=hgg^{-1}=h\in H$

    > ==Notation==<u>Remark</u>: 
    >
    > * Sometimes people write $N\lhd G$  to mean $N$ is a normal subgroup of $G$.
    > * People also write $H < G$ to mean $H$ is a subgroup of $G$.

3. $G$ is a group. 

    Define the <u>**center**</u> of $G$:  $Z(G)=\{ g\in G|\forall x\in G, gx=xg \}$

    (In particular, if $G$ is abelian, $Z(G)=G$)

    We'll verify $Z(G)$ is a subgroup of $G$:

    * $\forall a,b\in Z(G)$,  $\forall x\in G$. 

        $(ab)x = a(bx)=a(xb)=(ax)b=(xa)b = x(ab)$

        So $ab\in Z(G)$

    * $1\in Z(G): \forall x\in G, 1x = x1 = x$
    
    * $\forall a \in Z(G), \forall x\in G, ax = xa$.
    
        $a^{-1}(ax)a^{-1} = a^{-1}(xa)a^{-1}$
    
        $xa^{-1}=a^{-1}x$
    
        So $a^{-1}\in Z(G)$
    
    Next we'll verify $Z(G)$ is normal
    
    * $\forall a\in Z(G)$,  $\forall g\in G, $ $gag^{-1} = agg^{-1} = a\in Z(G)$



## Isomorphism





â€‹     